theories/typing/constrained.v
@@ -2,78 +2,6 @@ From refinedc.typing Require Export type.
 From refinedc.typing Require Import programs optional.
 Set Default Proof Using "Type".
 
-Section constrained.
-  Context `{!typeG Σ}.
-
-  Program Definition constrained (ty : type) (P : iProp Σ) : type := {|
-    ty_own β l := (l ◁ₗ{β} ty ∗ □ P)%I
-  |}.
-  Next Obligation. move => ty P ? l ?. iIntros "[H $]". by iApply ty_share. Qed.
-
-  Global Instance constrained_rty_ne n : Proper ((dist n) ==> (dist n) ==> (dist n)) constrained.
-  Proof. solve_type_proper. Qed.
-  Global Instance constrained_rty_proper : Proper ((≡) ==> (≡) ==> (≡)) constrained.
-  Proof. solve_type_proper. Qed.
-
-  Global Program Instance constrained_movable ty P `{!Movable ty} : Movable (constrained ty P) := {|
-     ty_layout := ty.(ty_layout);
-     ty_own_val v := (v ◁ᵥ ty ∗ □ P)%I;
-  |}.
-  Next Obligation. iIntros (????) "[? _]". by iApply ty_aligned. Qed.
-  Next Obligation. iIntros (????) "[? _]". by iApply ty_size_eq. Qed.
-  Next Obligation. iIntros (????) "[? $]". by iApply ty_deref. Qed.
-  Next Obligation. iIntros (??????) "Hl [? $]". by iApply (ty_ref with "[//] [Hl]"). Qed.
-
-  Global Instance constrained_loc_in_bounds ty β P `{!LocInBounds ty β} :
-    LocInBounds (constrained ty P) β.
-  Proof.
-    constructor. iIntros (l) "[Hl _]". by iApply loc_in_bounds_in_bounds.
-  Qed.
-
-  Lemma simplify_hyp_place_constrained P l β ty T `{!Persistent P}:
-    (P -∗ l ◁ₗ{β} ty -∗ T) -∗ simplify_hyp (l◁ₗ{β} constrained ty P) T.
-  Proof. iIntros "HT [Hl #?]". by iApply "HT". Qed.
-  Global Instance simplify_hyp_place_constrained_inst P l β ty `{!Persistent P}:
-    SimplifyHypPlace l β (constrained ty P)%I (Some 0%N) :=
-    λ T, i2p (simplify_hyp_place_constrained P l β ty T).
-
-  Lemma simplify_goal_place_constrained P l β ty T `{!Persistent P}:
-    T (l ◁ₗ{β} ty ∗ P) -∗ simplify_goal (l◁ₗ{β} constrained ty P) T.
-  Proof. iIntros "HT". iExists _. iFrame. iIntros "[$ #?]". by iModIntro. Qed.
-  Global Instance simplify_goal_place_constrained_inst P l β ty `{!Persistent P}:
-    SimplifyGoalPlace l β (constrained ty P)%I (Some 0%N) :=
-    λ T, i2p (simplify_goal_place_constrained P l β ty T).
-
-  Lemma simplify_hyp_val_constrained P v ty T `{!Movable ty}:
-    (P -∗ v ◁ᵥ ty -∗ T) -∗ simplify_hyp (v◁ᵥ constrained ty P) T.
-  Proof. iIntros "HT [Hl #?]". by iApply "HT". Qed.
-  Global Instance simplify_hyp_val_constrained_inst P v ty `{!Movable ty}:
-    SimplifyHypVal v (constrained ty P)%I (Some 0%N) :=
-    λ T, i2p (simplify_hyp_val_constrained P v ty T).
-
-  Lemma simplify_goal_val_constrained P v ty T `{!Movable ty} `{!Persistent P}:
-    T (v ◁ᵥ ty ∗ P) -∗ simplify_goal (v◁ᵥ constrained ty P) T.
-  Proof. iIntros "HT". iExists _. iFrame. iIntros "[$ #?]". by iModIntro. Qed.
-  Global Instance simplify_goal_val_constrained_inst P v ty `{!Movable ty} `{!Persistent P}:
-    SimplifyGoalVal v (constrained ty P)%I (Some 0%N) :=
-    λ T, i2p (simplify_goal_val_constrained P v ty T).
-
-  Global Program Instance constrained_optional ty P optty ot1 ot2 `{!Movable ty} `{!Movable optty} `{!Optionable ty optty ot1 ot2} : Optionable (constrained ty P) optty ot1 ot2 := {|
-    opt_pre v1 v2 := opt_pre ty v1 v2
-  |}.
-  Next Obligation. move => ???????? /=. apply opt_alt_sz. Qed.
-  Next Obligation.
-    iIntros (????????[]?????) "Hpre H1 H2". 1: iDestruct "H1" as "[H1 _]".
-    by iApply (opt_bin_op true with "Hpre H1 H2").
-    by iApply (opt_bin_op false with "Hpre H1 H2").
-  Qed.
-
-  Global Instance optionable_agree_constrained P (ty2 : type) `{!OptionableAgree ty1 ty2} : OptionableAgree (constrained ty1 P) ty2.
-  Proof. done. Qed.
-End constrained.
-Typeclasses Opaque constrained.
-
-
 Class OwnConstraint `{!typeG Σ} (P : own_state → iProp Σ) : Prop := {
   own_constraint_persistent : Persistent (P Shr);
   own_constraint_share E : ↑shrN ⊆ E → P Own ={E}=∗ P Shr;
@@ -83,7 +11,7 @@ Global Existing Instance own_constraint_persistent.
 Section own_constrained.
   Context `{!typeG Σ}.
 
-  Program Definition own_constrained (ty : type) (P : own_state → iProp Σ) `{!OwnConstraint P} : type := {|
+  Program Definition own_constrained (P : own_state → iProp Σ) `{!OwnConstraint P} (ty : type) : type := {|
     ty_own β l := (l ◁ₗ{β} ty ∗ P β)%I
   |}.
   Next Obligation.
@@ -92,7 +20,12 @@ Section own_constrained.
     by iApply own_constraint_share.
   Qed.
 
-  Global Program Instance own_constrained_movable ty P `{!Movable ty}  `{!OwnConstraint P} : Movable (own_constrained ty P) := {|
+  Global Instance own_constrained_rty_ne n P `{!OwnConstraint P} : Proper ((dist n) ==> (dist n)) (own_constrained P).
+  Proof. solve_type_proper. Qed.
+  Global Instance own_constrained_rty_proper P `{!OwnConstraint P} : Proper ((≡) ==> (≡)) (own_constrained P).
+  Proof. solve_type_proper. Qed.
+
+  Global Program Instance own_constrained_movable ty P `{!Movable ty} `{!OwnConstraint P} : Movable (own_constrained P ty) := {|
      ty_layout := ty.(ty_layout);
      ty_own_val v := (v ◁ᵥ ty ∗ P Own)%I;
   |}.
@@ -101,33 +34,52 @@ Section own_constrained.
   Next Obligation. iIntros (?????) "[? $]". by iApply ty_deref. Qed.
   Next Obligation. iIntros (???????) "Hl [? $]". by iApply (ty_ref with "[//] [Hl]"). Qed.
 
+  Global Instance own_constrained_loc_in_bounds ty β P `{!OwnConstraint P} `{!LocInBounds ty β} :
+    LocInBounds (own_constrained P ty) β.
+  Proof.
+    constructor. iIntros (l) "[Hl _]". by iApply loc_in_bounds_in_bounds.
+  Qed.
+
   Lemma simplify_hyp_place_own_constrained P l β ty T `{!OwnConstraint P}:
-    (P β -∗ l ◁ₗ{β} ty -∗ T) -∗ simplify_hyp (l◁ₗ{β} own_constrained ty P) T.
+    (P β -∗ l ◁ₗ{β} ty -∗ T) -∗ simplify_hyp (l◁ₗ{β} own_constrained P ty) T.
   Proof. iIntros "HT [Hl HP]". by iApply ("HT" with "HP"). Qed.
   Global Instance simplify_hyp_place_own_constrained_inst P l β ty `{!OwnConstraint P}:
-    SimplifyHypPlace l β (own_constrained ty P)%I (Some 0%N) :=
+    SimplifyHypPlace l β (own_constrained P ty)%I (Some 0%N) :=
     λ T, i2p (simplify_hyp_place_own_constrained P l β ty T).
 
   Lemma simplify_goal_place_own_constrained P l β ty T `{!OwnConstraint P}:
-    T (l ◁ₗ{β} ty ∗ P β) -∗ simplify_goal (l◁ₗ{β} own_constrained ty P) T.
+    T (l ◁ₗ{β} ty ∗ P β) -∗ simplify_goal (l◁ₗ{β} own_constrained P ty) T.
   Proof. iIntros "HT". iExists _. iFrame. iIntros "[$ $]". Qed.
   Global Instance simplify_goal_place_own_constrained_inst P l β ty `{!OwnConstraint P}:
-    SimplifyGoalPlace l β (own_constrained ty P)%I (Some 0%N) :=
+    SimplifyGoalPlace l β (own_constrained P ty)%I (Some 0%N) :=
     λ T, i2p (simplify_goal_place_own_constrained P l β ty T).
 
   Lemma simplify_hyp_val_own_constrained P v ty T `{!Movable ty} `{!OwnConstraint P}:
-    (P Own -∗ v ◁ᵥ ty -∗ T) -∗ simplify_hyp (v ◁ᵥ own_constrained ty P) T.
+    (P Own -∗ v ◁ᵥ ty -∗ T) -∗ simplify_hyp (v ◁ᵥ own_constrained P ty) T.
   Proof. iIntros "HT [Hl HP]". by iApply ("HT" with "HP"). Qed.
   Global Instance simplify_hyp_val_own_constrained_inst P v ty `{!Movable ty} `{!OwnConstraint P}:
-    SimplifyHypVal v (own_constrained ty P)%I (Some 0%N) :=
+    SimplifyHypVal v (own_constrained P ty)%I (Some 0%N) :=
     λ T, i2p (simplify_hyp_val_own_constrained P v ty T).
 
   Lemma simplify_goal_val_own_constrained P v ty T `{!Movable ty} `{!OwnConstraint P}:
-    T (v ◁ᵥ ty ∗ P Own) -∗ simplify_goal (v ◁ᵥ own_constrained ty P) T.
+    T (v ◁ᵥ ty ∗ P Own) -∗ simplify_goal (v ◁ᵥ own_constrained P ty) T.
   Proof. iIntros "HT". iExists _. iFrame. iIntros "[$ $]". Qed.
   Global Instance simplify_goal_val_own_constrained_inst P v ty `{!Movable ty} `{!OwnConstraint P}:
-    SimplifyGoalVal v (own_constrained ty P)%I (Some 0%N) :=
+    SimplifyGoalVal v (own_constrained P ty)%I (Some 0%N) :=
     λ T, i2p (simplify_goal_val_own_constrained P v ty T).
+
+  Global Program Instance own_constrained_optional ty P optty ot1 ot2 `{!Movable ty} `{!Movable optty} `{!OwnConstraint P} `{!Optionable ty optty ot1 ot2} : Optionable (own_constrained P ty) optty ot1 ot2 := {|
+    opt_pre v1 v2 := opt_pre ty v1 v2
+  |}.
+  Next Obligation. move => ????????? /=. apply opt_alt_sz. Qed.
+  Next Obligation.
+    iIntros (?????????[]?????) "Hpre H1 H2". 1: iDestruct "H1" as "[H1 _]".
+    by iApply (opt_bin_op true with "Hpre H1 H2").
+    by iApply (opt_bin_op false with "Hpre H1 H2").
+  Qed.
+
+  Global Instance optionable_agree_own_constrained P (ty2 : type) `{!OwnConstraint P} `{!OptionableAgree ty1 ty2} : OptionableAgree (own_constrained P ty1) ty2.
+  Proof. done. Qed.
 
 
   Definition tyown_constraint (l : loc) (ty : type) (β : own_state) : iProp Σ := l ◁ₗ{β} ty.
@@ -149,5 +101,62 @@ Section own_constrained.
     SimplifyGoal (tyown_constraint l ty β) (Some 0%N) :=
     λ T, i2p (simplify_goal_place_tyown_constrained l β ty T).
 End own_constrained.
+
 Typeclasses Opaque own_constrained tyown_constraint.
 Arguments tyown_constraint : simpl never.
+
+Section constrained.
+  Context `{!typeG Σ}.
+
+  Definition persistent_own_constraint (P : iProp Σ) (β : own_state) : iProp Σ := □ P.
+
+  Global Instance persistent_own_constraint_inst P: OwnConstraint (persistent_own_constraint P).
+  Proof. constructor; [by apply _ | by iIntros (??) "H !>"]. Qed.
+
+  Lemma simplify_hyp_place_persistent_constrained P β T:
+    (P -∗ T) -∗ simplify_hyp (persistent_own_constraint P β) T.
+  Proof. iIntros "HT #Hl". by iApply "HT". Qed.
+  Global Instance simplify_hyp_place_persistent_constrained_inst P β:
+    SimplifyHyp (persistent_own_constraint P β) (Some 0%N) :=
+    λ T, i2p (simplify_hyp_place_persistent_constrained P β T).
+
+  Lemma simplify_goal_place_persistent_constrained P `{!Persistent P} β T:
+    T P -∗ simplify_goal (persistent_own_constraint P β) T.
+  Proof. iIntros "HT". iExists _. iFrame. iIntros "#$". Qed.
+  Global Instance simplify_goal_place_persistent_constrained_inst P `{!Persistent P} β:
+    SimplifyGoal (persistent_own_constraint P β) (Some 0%N) :=
+    λ T, i2p (simplify_goal_place_persistent_constrained P β T).
+End constrained.
+
+Typeclasses Opaque persistent_own_constraint.
+Arguments persistent_own_constraint : simpl never.
+
+Notation constrained ty P := (own_constrained (persistent_own_constraint P) ty).
+
+Section nonshr_constrained.
+  Context `{!typeG Σ}.
+
+  Definition nonshr_constraint (P : iProp Σ) (β : own_state) : iProp Σ :=
+    match β with | Own => P | Shr => True end.
+
+  Global Program Instance nonshr_constraint_own_constraint P: OwnConstraint (nonshr_constraint P).
+  Next Obligation. iIntros (???) "?". done. Qed.
+
+  Lemma simplify_hyp_place_nonshr_constrained P T:
+    (P -∗ T) -∗ simplify_hyp (nonshr_constraint P Own) T.
+  Proof. iIntros "HT Hl". by iApply "HT". Qed.
+  Global Instance simplify_hyp_place_nonshr_constrained_inst P:
+    SimplifyHyp (nonshr_constraint P Own) (Some 0%N) :=
+    λ T, i2p (simplify_hyp_place_nonshr_constrained P T).
+
+  Lemma simplify_goal_place_nonshr_constrained P T:
+    T P -∗ simplify_goal (nonshr_constraint P Own) T.
+  Proof. iIntros "HT". iExists _. iFrame. iIntros "$". Qed.
+  Global Instance simplify_goal_place_nonshr_constrained_inst P:
+    SimplifyGoal (nonshr_constraint P Own) (Some 0%N) :=
+    λ T, i2p (simplify_goal_place_nonshr_constrained P T).
+
+End nonshr_constrained.
+
+Typeclasses Opaque nonshr_constraint.
+Arguments nonshr_constraint : simpl never.
