tutorial/proofs/t03_list/generated_code.v
@@ -6,163 +6,163 @@ Set Default Proof Using "Type".
 (* Generated from [tutorial/t03_list.c]. *)
 Section code.
   Definition file_0 : string := "tutorial/t03_list.c".
-  Definition loc_2 : location_info := LocationInfo file_0 154 4 154 25.
-  Definition loc_3 : location_info := LocationInfo file_0 155 4 155 42.
-  Definition loc_4 : location_info := LocationInfo file_0 156 4 156 42.
-  Definition loc_5 : location_info := LocationInfo file_0 157 4 157 42.
-  Definition loc_6 : location_info := LocationInfo file_0 159 4 159 28.
-  Definition loc_7 : location_info := LocationInfo file_0 161 4 161 15.
-  Definition loc_8 : location_info := LocationInfo file_0 162 4 162 15.
-  Definition loc_9 : location_info := LocationInfo file_0 163 4 163 15.
-  Definition loc_10 : location_info := LocationInfo file_0 165 4 165 29.
-  Definition loc_11 : location_info := LocationInfo file_0 166 4 166 29.
-  Definition loc_12 : location_info := LocationInfo file_0 167 4 167 29.
-  Definition loc_13 : location_info := LocationInfo file_0 169 4 169 29.
-  Definition loc_14 : location_info := LocationInfo file_0 171 4 171 25.
-  Definition loc_15 : location_info := LocationInfo file_0 173 4 173 29.
-  Definition loc_16 : location_info := LocationInfo file_0 175 4 175 23.
-  Definition loc_17 : location_info := LocationInfo file_0 176 4 176 23.
-  Definition loc_18 : location_info := LocationInfo file_0 177 4 177 23.
-  Definition loc_19 : location_info := LocationInfo file_0 179 4 179 28.
-  Definition loc_20 : location_info := LocationInfo file_0 181 4 181 32.
-  Definition loc_21 : location_info := LocationInfo file_0 182 4 182 32.
-  Definition loc_22 : location_info := LocationInfo file_0 183 4 183 32.
-  Definition loc_23 : location_info := LocationInfo file_0 185 4 185 32.
-  Definition loc_24 : location_info := LocationInfo file_0 186 4 186 32.
-  Definition loc_25 : location_info := LocationInfo file_0 187 4 187 32.
-  Definition loc_26 : location_info := LocationInfo file_0 187 4 187 8.
-  Definition loc_27 : location_info := LocationInfo file_0 187 4 187 8.
-  Definition loc_28 : location_info := LocationInfo file_0 187 9 187 23.
-  Definition loc_29 : location_info := LocationInfo file_0 187 25 187 30.
-  Definition loc_30 : location_info := LocationInfo file_0 187 25 187 30.
-  Definition loc_31 : location_info := LocationInfo file_0 186 4 186 8.
-  Definition loc_32 : location_info := LocationInfo file_0 186 4 186 8.
-  Definition loc_33 : location_info := LocationInfo file_0 186 9 186 23.
-  Definition loc_34 : location_info := LocationInfo file_0 186 25 186 30.
-  Definition loc_35 : location_info := LocationInfo file_0 186 25 186 30.
-  Definition loc_36 : location_info := LocationInfo file_0 185 4 185 8.
-  Definition loc_37 : location_info := LocationInfo file_0 185 4 185 8.
-  Definition loc_38 : location_info := LocationInfo file_0 185 9 185 23.
-  Definition loc_39 : location_info := LocationInfo file_0 185 25 185 30.
-  Definition loc_40 : location_info := LocationInfo file_0 185 25 185 30.
-  Definition loc_41 : location_info := LocationInfo file_0 183 11 183 30.
-  Definition loc_42 : location_info := LocationInfo file_0 183 11 183 17.
-  Definition loc_43 : location_info := LocationInfo file_0 183 11 183 17.
-  Definition loc_44 : location_info := LocationInfo file_0 183 12 183 17.
-  Definition loc_45 : location_info := LocationInfo file_0 183 12 183 17.
-  Definition loc_46 : location_info := LocationInfo file_0 183 21 183 30.
-  Definition loc_47 : location_info := LocationInfo file_0 183 29 183 30.
-  Definition loc_48 : location_info := LocationInfo file_0 182 11 182 30.
-  Definition loc_49 : location_info := LocationInfo file_0 182 11 182 17.
-  Definition loc_50 : location_info := LocationInfo file_0 182 11 182 17.
-  Definition loc_51 : location_info := LocationInfo file_0 182 12 182 17.
-  Definition loc_52 : location_info := LocationInfo file_0 182 12 182 17.
-  Definition loc_53 : location_info := LocationInfo file_0 182 21 182 30.
-  Definition loc_54 : location_info := LocationInfo file_0 182 29 182 30.
-  Definition loc_55 : location_info := LocationInfo file_0 181 11 181 30.
-  Definition loc_56 : location_info := LocationInfo file_0 181 11 181 17.
-  Definition loc_57 : location_info := LocationInfo file_0 181 11 181 17.
-  Definition loc_58 : location_info := LocationInfo file_0 181 12 181 17.
-  Definition loc_59 : location_info := LocationInfo file_0 181 12 181 17.
-  Definition loc_60 : location_info := LocationInfo file_0 181 21 181 30.
-  Definition loc_61 : location_info := LocationInfo file_0 181 29 181 30.
-  Definition loc_62 : location_info := LocationInfo file_0 179 11 179 26.
-  Definition loc_63 : location_info := LocationInfo file_0 179 11 179 19.
-  Definition loc_64 : location_info := LocationInfo file_0 179 11 179 19.
-  Definition loc_65 : location_info := LocationInfo file_0 179 20 179 25.
-  Definition loc_66 : location_info := LocationInfo file_0 179 21 179 25.
-  Definition loc_67 : location_info := LocationInfo file_0 177 4 177 9.
-  Definition loc_68 : location_info := LocationInfo file_0 177 12 177 22.
-  Definition loc_69 : location_info := LocationInfo file_0 177 12 177 15.
-  Definition loc_70 : location_info := LocationInfo file_0 177 12 177 15.
-  Definition loc_71 : location_info := LocationInfo file_0 177 16 177 21.
-  Definition loc_72 : location_info := LocationInfo file_0 177 17 177 21.
-  Definition loc_73 : location_info := LocationInfo file_0 176 4 176 9.
-  Definition loc_74 : location_info := LocationInfo file_0 176 12 176 22.
-  Definition loc_75 : location_info := LocationInfo file_0 176 12 176 15.
-  Definition loc_76 : location_info := LocationInfo file_0 176 12 176 15.
-  Definition loc_77 : location_info := LocationInfo file_0 176 16 176 21.
-  Definition loc_78 : location_info := LocationInfo file_0 176 17 176 21.
-  Definition loc_79 : location_info := LocationInfo file_0 175 4 175 9.
-  Definition loc_80 : location_info := LocationInfo file_0 175 12 175 22.
-  Definition loc_81 : location_info := LocationInfo file_0 175 12 175 15.
-  Definition loc_82 : location_info := LocationInfo file_0 175 12 175 15.
-  Definition loc_83 : location_info := LocationInfo file_0 175 16 175 21.
-  Definition loc_84 : location_info := LocationInfo file_0 175 17 175 21.
-  Definition loc_85 : location_info := LocationInfo file_0 173 11 173 27.
-  Definition loc_86 : location_info := LocationInfo file_0 173 11 173 17.
-  Definition loc_87 : location_info := LocationInfo file_0 173 11 173 17.
-  Definition loc_88 : location_info := LocationInfo file_0 173 18 173 23.
-  Definition loc_89 : location_info := LocationInfo file_0 173 19 173 23.
-  Definition loc_90 : location_info := LocationInfo file_0 173 25 173 26.
-  Definition loc_91 : location_info := LocationInfo file_0 171 4 171 8.
-  Definition loc_92 : location_info := LocationInfo file_0 171 11 171 24.
-  Definition loc_93 : location_info := LocationInfo file_0 171 11 171 18.
-  Definition loc_94 : location_info := LocationInfo file_0 171 11 171 18.
-  Definition loc_95 : location_info := LocationInfo file_0 171 19 171 23.
-  Definition loc_96 : location_info := LocationInfo file_0 171 19 171 23.
-  Definition loc_97 : location_info := LocationInfo file_0 169 11 169 27.
-  Definition loc_98 : location_info := LocationInfo file_0 169 11 169 17.
-  Definition loc_99 : location_info := LocationInfo file_0 169 11 169 17.
-  Definition loc_100 : location_info := LocationInfo file_0 169 18 169 23.
-  Definition loc_101 : location_info := LocationInfo file_0 169 19 169 23.
-  Definition loc_102 : location_info := LocationInfo file_0 169 25 169 26.
-  Definition loc_103 : location_info := LocationInfo file_0 167 4 167 8.
-  Definition loc_104 : location_info := LocationInfo file_0 167 11 167 28.
-  Definition loc_105 : location_info := LocationInfo file_0 167 11 167 15.
-  Definition loc_106 : location_info := LocationInfo file_0 167 11 167 15.
-  Definition loc_107 : location_info := LocationInfo file_0 167 16 167 20.
-  Definition loc_108 : location_info := LocationInfo file_0 167 16 167 20.
-  Definition loc_109 : location_info := LocationInfo file_0 167 22 167 27.
-  Definition loc_110 : location_info := LocationInfo file_0 167 22 167 27.
-  Definition loc_111 : location_info := LocationInfo file_0 166 4 166 8.
-  Definition loc_112 : location_info := LocationInfo file_0 166 11 166 28.
-  Definition loc_113 : location_info := LocationInfo file_0 166 11 166 15.
-  Definition loc_114 : location_info := LocationInfo file_0 166 11 166 15.
-  Definition loc_115 : location_info := LocationInfo file_0 166 16 166 20.
-  Definition loc_116 : location_info := LocationInfo file_0 166 16 166 20.
-  Definition loc_117 : location_info := LocationInfo file_0 166 22 166 27.
-  Definition loc_118 : location_info := LocationInfo file_0 166 22 166 27.
-  Definition loc_119 : location_info := LocationInfo file_0 165 4 165 8.
-  Definition loc_120 : location_info := LocationInfo file_0 165 11 165 28.
-  Definition loc_121 : location_info := LocationInfo file_0 165 11 165 15.
-  Definition loc_122 : location_info := LocationInfo file_0 165 11 165 15.
-  Definition loc_123 : location_info := LocationInfo file_0 165 16 165 20.
-  Definition loc_124 : location_info := LocationInfo file_0 165 16 165 20.
-  Definition loc_125 : location_info := LocationInfo file_0 165 22 165 27.
-  Definition loc_126 : location_info := LocationInfo file_0 165 22 165 27.
-  Definition loc_127 : location_info := LocationInfo file_0 163 4 163 10.
-  Definition loc_128 : location_info := LocationInfo file_0 163 5 163 10.
-  Definition loc_129 : location_info := LocationInfo file_0 163 5 163 10.
-  Definition loc_130 : location_info := LocationInfo file_0 163 13 163 14.
-  Definition loc_131 : location_info := LocationInfo file_0 162 4 162 10.
-  Definition loc_132 : location_info := LocationInfo file_0 162 5 162 10.
-  Definition loc_133 : location_info := LocationInfo file_0 162 5 162 10.
-  Definition loc_134 : location_info := LocationInfo file_0 162 13 162 14.
-  Definition loc_135 : location_info := LocationInfo file_0 161 4 161 10.
-  Definition loc_136 : location_info := LocationInfo file_0 161 5 161 10.
-  Definition loc_137 : location_info := LocationInfo file_0 161 5 161 10.
-  Definition loc_138 : location_info := LocationInfo file_0 161 13 161 14.
-  Definition loc_139 : location_info := LocationInfo file_0 159 11 159 26.
-  Definition loc_140 : location_info := LocationInfo file_0 159 11 159 19.
-  Definition loc_141 : location_info := LocationInfo file_0 159 11 159 19.
-  Definition loc_142 : location_info := LocationInfo file_0 159 20 159 25.
-  Definition loc_143 : location_info := LocationInfo file_0 159 21 159 25.
-  Definition loc_144 : location_info := LocationInfo file_0 157 20 157 41.
-  Definition loc_145 : location_info := LocationInfo file_0 157 20 157 25.
-  Definition loc_146 : location_info := LocationInfo file_0 157 20 157 25.
-  Definition loc_147 : location_info := LocationInfo file_0 157 26 157 40.
-  Definition loc_150 : location_info := LocationInfo file_0 156 20 156 41.
-  Definition loc_151 : location_info := LocationInfo file_0 156 20 156 25.
-  Definition loc_152 : location_info := LocationInfo file_0 156 20 156 25.
-  Definition loc_153 : location_info := LocationInfo file_0 156 26 156 40.
-  Definition loc_156 : location_info := LocationInfo file_0 155 20 155 41.
-  Definition loc_157 : location_info := LocationInfo file_0 155 20 155 25.
-  Definition loc_158 : location_info := LocationInfo file_0 155 20 155 25.
-  Definition loc_159 : location_info := LocationInfo file_0 155 26 155 40.
-  Definition loc_162 : location_info := LocationInfo file_0 154 18 154 24.
-  Definition loc_163 : location_info := LocationInfo file_0 154 18 154 22.
-  Definition loc_164 : location_info := LocationInfo file_0 154 18 154 22.
+  Definition loc_2 : location_info := LocationInfo file_0 173 4 173 25.
+  Definition loc_3 : location_info := LocationInfo file_0 174 4 174 42.
+  Definition loc_4 : location_info := LocationInfo file_0 175 4 175 42.
+  Definition loc_5 : location_info := LocationInfo file_0 176 4 176 42.
+  Definition loc_6 : location_info := LocationInfo file_0 178 4 178 28.
+  Definition loc_7 : location_info := LocationInfo file_0 180 4 180 15.
+  Definition loc_8 : location_info := LocationInfo file_0 181 4 181 15.
+  Definition loc_9 : location_info := LocationInfo file_0 182 4 182 15.
+  Definition loc_10 : location_info := LocationInfo file_0 184 4 184 29.
+  Definition loc_11 : location_info := LocationInfo file_0 185 4 185 29.
+  Definition loc_12 : location_info := LocationInfo file_0 186 4 186 29.
+  Definition loc_13 : location_info := LocationInfo file_0 188 4 188 29.
+  Definition loc_14 : location_info := LocationInfo file_0 190 4 190 25.
+  Definition loc_15 : location_info := LocationInfo file_0 192 4 192 29.
+  Definition loc_16 : location_info := LocationInfo file_0 194 4 194 23.
+  Definition loc_17 : location_info := LocationInfo file_0 195 4 195 23.
+  Definition loc_18 : location_info := LocationInfo file_0 196 4 196 23.
+  Definition loc_19 : location_info := LocationInfo file_0 198 4 198 28.
+  Definition loc_20 : location_info := LocationInfo file_0 200 4 200 32.
+  Definition loc_21 : location_info := LocationInfo file_0 201 4 201 32.
+  Definition loc_22 : location_info := LocationInfo file_0 202 4 202 32.
+  Definition loc_23 : location_info := LocationInfo file_0 204 4 204 32.
+  Definition loc_24 : location_info := LocationInfo file_0 205 4 205 32.
+  Definition loc_25 : location_info := LocationInfo file_0 206 4 206 32.
+  Definition loc_26 : location_info := LocationInfo file_0 206 4 206 8.
+  Definition loc_27 : location_info := LocationInfo file_0 206 4 206 8.
+  Definition loc_28 : location_info := LocationInfo file_0 206 9 206 23.
+  Definition loc_29 : location_info := LocationInfo file_0 206 25 206 30.
+  Definition loc_30 : location_info := LocationInfo file_0 206 25 206 30.
+  Definition loc_31 : location_info := LocationInfo file_0 205 4 205 8.
+  Definition loc_32 : location_info := LocationInfo file_0 205 4 205 8.
+  Definition loc_33 : location_info := LocationInfo file_0 205 9 205 23.
+  Definition loc_34 : location_info := LocationInfo file_0 205 25 205 30.
+  Definition loc_35 : location_info := LocationInfo file_0 205 25 205 30.
+  Definition loc_36 : location_info := LocationInfo file_0 204 4 204 8.
+  Definition loc_37 : location_info := LocationInfo file_0 204 4 204 8.
+  Definition loc_38 : location_info := LocationInfo file_0 204 9 204 23.
+  Definition loc_39 : location_info := LocationInfo file_0 204 25 204 30.
+  Definition loc_40 : location_info := LocationInfo file_0 204 25 204 30.
+  Definition loc_41 : location_info := LocationInfo file_0 202 11 202 30.
+  Definition loc_42 : location_info := LocationInfo file_0 202 11 202 17.
+  Definition loc_43 : location_info := LocationInfo file_0 202 11 202 17.
+  Definition loc_44 : location_info := LocationInfo file_0 202 12 202 17.
+  Definition loc_45 : location_info := LocationInfo file_0 202 12 202 17.
+  Definition loc_46 : location_info := LocationInfo file_0 202 21 202 30.
+  Definition loc_47 : location_info := LocationInfo file_0 202 29 202 30.
+  Definition loc_48 : location_info := LocationInfo file_0 201 11 201 30.
+  Definition loc_49 : location_info := LocationInfo file_0 201 11 201 17.
+  Definition loc_50 : location_info := LocationInfo file_0 201 11 201 17.
+  Definition loc_51 : location_info := LocationInfo file_0 201 12 201 17.
+  Definition loc_52 : location_info := LocationInfo file_0 201 12 201 17.
+  Definition loc_53 : location_info := LocationInfo file_0 201 21 201 30.
+  Definition loc_54 : location_info := LocationInfo file_0 201 29 201 30.
+  Definition loc_55 : location_info := LocationInfo file_0 200 11 200 30.
+  Definition loc_56 : location_info := LocationInfo file_0 200 11 200 17.
+  Definition loc_57 : location_info := LocationInfo file_0 200 11 200 17.
+  Definition loc_58 : location_info := LocationInfo file_0 200 12 200 17.
+  Definition loc_59 : location_info := LocationInfo file_0 200 12 200 17.
+  Definition loc_60 : location_info := LocationInfo file_0 200 21 200 30.
+  Definition loc_61 : location_info := LocationInfo file_0 200 29 200 30.
+  Definition loc_62 : location_info := LocationInfo file_0 198 11 198 26.
+  Definition loc_63 : location_info := LocationInfo file_0 198 11 198 19.
+  Definition loc_64 : location_info := LocationInfo file_0 198 11 198 19.
+  Definition loc_65 : location_info := LocationInfo file_0 198 20 198 25.
+  Definition loc_66 : location_info := LocationInfo file_0 198 21 198 25.
+  Definition loc_67 : location_info := LocationInfo file_0 196 4 196 9.
+  Definition loc_68 : location_info := LocationInfo file_0 196 12 196 22.
+  Definition loc_69 : location_info := LocationInfo file_0 196 12 196 15.
+  Definition loc_70 : location_info := LocationInfo file_0 196 12 196 15.
+  Definition loc_71 : location_info := LocationInfo file_0 196 16 196 21.
+  Definition loc_72 : location_info := LocationInfo file_0 196 17 196 21.
+  Definition loc_73 : location_info := LocationInfo file_0 195 4 195 9.
+  Definition loc_74 : location_info := LocationInfo file_0 195 12 195 22.
+  Definition loc_75 : location_info := LocationInfo file_0 195 12 195 15.
+  Definition loc_76 : location_info := LocationInfo file_0 195 12 195 15.
+  Definition loc_77 : location_info := LocationInfo file_0 195 16 195 21.
+  Definition loc_78 : location_info := LocationInfo file_0 195 17 195 21.
+  Definition loc_79 : location_info := LocationInfo file_0 194 4 194 9.
+  Definition loc_80 : location_info := LocationInfo file_0 194 12 194 22.
+  Definition loc_81 : location_info := LocationInfo file_0 194 12 194 15.
+  Definition loc_82 : location_info := LocationInfo file_0 194 12 194 15.
+  Definition loc_83 : location_info := LocationInfo file_0 194 16 194 21.
+  Definition loc_84 : location_info := LocationInfo file_0 194 17 194 21.
+  Definition loc_85 : location_info := LocationInfo file_0 192 11 192 27.
+  Definition loc_86 : location_info := LocationInfo file_0 192 11 192 17.
+  Definition loc_87 : location_info := LocationInfo file_0 192 11 192 17.
+  Definition loc_88 : location_info := LocationInfo file_0 192 18 192 23.
+  Definition loc_89 : location_info := LocationInfo file_0 192 19 192 23.
+  Definition loc_90 : location_info := LocationInfo file_0 192 25 192 26.
+  Definition loc_91 : location_info := LocationInfo file_0 190 4 190 8.
+  Definition loc_92 : location_info := LocationInfo file_0 190 11 190 24.
+  Definition loc_93 : location_info := LocationInfo file_0 190 11 190 18.
+  Definition loc_94 : location_info := LocationInfo file_0 190 11 190 18.
+  Definition loc_95 : location_info := LocationInfo file_0 190 19 190 23.
+  Definition loc_96 : location_info := LocationInfo file_0 190 19 190 23.
+  Definition loc_97 : location_info := LocationInfo file_0 188 11 188 27.
+  Definition loc_98 : location_info := LocationInfo file_0 188 11 188 17.
+  Definition loc_99 : location_info := LocationInfo file_0 188 11 188 17.
+  Definition loc_100 : location_info := LocationInfo file_0 188 18 188 23.
+  Definition loc_101 : location_info := LocationInfo file_0 188 19 188 23.
+  Definition loc_102 : location_info := LocationInfo file_0 188 25 188 26.
+  Definition loc_103 : location_info := LocationInfo file_0 186 4 186 8.
+  Definition loc_104 : location_info := LocationInfo file_0 186 11 186 28.
+  Definition loc_105 : location_info := LocationInfo file_0 186 11 186 15.
+  Definition loc_106 : location_info := LocationInfo file_0 186 11 186 15.
+  Definition loc_107 : location_info := LocationInfo file_0 186 16 186 20.
+  Definition loc_108 : location_info := LocationInfo file_0 186 16 186 20.
+  Definition loc_109 : location_info := LocationInfo file_0 186 22 186 27.
+  Definition loc_110 : location_info := LocationInfo file_0 186 22 186 27.
+  Definition loc_111 : location_info := LocationInfo file_0 185 4 185 8.
+  Definition loc_112 : location_info := LocationInfo file_0 185 11 185 28.
+  Definition loc_113 : location_info := LocationInfo file_0 185 11 185 15.
+  Definition loc_114 : location_info := LocationInfo file_0 185 11 185 15.
+  Definition loc_115 : location_info := LocationInfo file_0 185 16 185 20.
+  Definition loc_116 : location_info := LocationInfo file_0 185 16 185 20.
+  Definition loc_117 : location_info := LocationInfo file_0 185 22 185 27.
+  Definition loc_118 : location_info := LocationInfo file_0 185 22 185 27.
+  Definition loc_119 : location_info := LocationInfo file_0 184 4 184 8.
+  Definition loc_120 : location_info := LocationInfo file_0 184 11 184 28.
+  Definition loc_121 : location_info := LocationInfo file_0 184 11 184 15.
+  Definition loc_122 : location_info := LocationInfo file_0 184 11 184 15.
+  Definition loc_123 : location_info := LocationInfo file_0 184 16 184 20.
+  Definition loc_124 : location_info := LocationInfo file_0 184 16 184 20.
+  Definition loc_125 : location_info := LocationInfo file_0 184 22 184 27.
+  Definition loc_126 : location_info := LocationInfo file_0 184 22 184 27.
+  Definition loc_127 : location_info := LocationInfo file_0 182 4 182 10.
+  Definition loc_128 : location_info := LocationInfo file_0 182 5 182 10.
+  Definition loc_129 : location_info := LocationInfo file_0 182 5 182 10.
+  Definition loc_130 : location_info := LocationInfo file_0 182 13 182 14.
+  Definition loc_131 : location_info := LocationInfo file_0 181 4 181 10.
+  Definition loc_132 : location_info := LocationInfo file_0 181 5 181 10.
+  Definition loc_133 : location_info := LocationInfo file_0 181 5 181 10.
+  Definition loc_134 : location_info := LocationInfo file_0 181 13 181 14.
+  Definition loc_135 : location_info := LocationInfo file_0 180 4 180 10.
+  Definition loc_136 : location_info := LocationInfo file_0 180 5 180 10.
+  Definition loc_137 : location_info := LocationInfo file_0 180 5 180 10.
+  Definition loc_138 : location_info := LocationInfo file_0 180 13 180 14.
+  Definition loc_139 : location_info := LocationInfo file_0 178 11 178 26.
+  Definition loc_140 : location_info := LocationInfo file_0 178 11 178 19.
+  Definition loc_141 : location_info := LocationInfo file_0 178 11 178 19.
+  Definition loc_142 : location_info := LocationInfo file_0 178 20 178 25.
+  Definition loc_143 : location_info := LocationInfo file_0 178 21 178 25.
+  Definition loc_144 : location_info := LocationInfo file_0 176 20 176 41.
+  Definition loc_145 : location_info := LocationInfo file_0 176 20 176 25.
+  Definition loc_146 : location_info := LocationInfo file_0 176 20 176 25.
+  Definition loc_147 : location_info := LocationInfo file_0 176 26 176 40.
+  Definition loc_150 : location_info := LocationInfo file_0 175 20 175 41.
+  Definition loc_151 : location_info := LocationInfo file_0 175 20 175 25.
+  Definition loc_152 : location_info := LocationInfo file_0 175 20 175 25.
+  Definition loc_153 : location_info := LocationInfo file_0 175 26 175 40.
+  Definition loc_156 : location_info := LocationInfo file_0 174 20 174 41.
+  Definition loc_157 : location_info := LocationInfo file_0 174 20 174 25.
+  Definition loc_158 : location_info := LocationInfo file_0 174 20 174 25.
+  Definition loc_159 : location_info := LocationInfo file_0 174 26 174 40.
+  Definition loc_162 : location_info := LocationInfo file_0 173 18 173 24.
+  Definition loc_163 : location_info := LocationInfo file_0 173 18 173 22.
+  Definition loc_164 : location_info := LocationInfo file_0 173 18 173 22.
   Definition loc_169 : location_info := LocationInfo file_0 27 4 27 26.
   Definition loc_170 : location_info := LocationInfo file_0 27 11 27 25.
   Definition loc_173 : location_info := LocationInfo file_0 35 4 35 32.
@@ -312,113 +312,139 @@ Section code.
   Definition loc_337 : location_info := LocationInfo file_0 107 5 107 6.
   Definition loc_338 : location_info := LocationInfo file_0 107 5 107 6.
   Definition loc_339 : location_info := LocationInfo file_0 107 10 107 24.
-  Definition loc_342 : location_info := LocationInfo file_0 117 2 117 19.
-  Definition loc_343 : location_info := LocationInfo file_0 121 2 123 3.
-  Definition loc_344 : location_info := LocationInfo file_0 124 2 124 12.
-  Definition loc_345 : location_info := LocationInfo file_0 124 2 124 6.
-  Definition loc_346 : location_info := LocationInfo file_0 124 3 124 6.
-  Definition loc_347 : location_info := LocationInfo file_0 124 3 124 6.
-  Definition loc_348 : location_info := LocationInfo file_0 124 9 124 11.
-  Definition loc_349 : location_info := LocationInfo file_0 124 9 124 11.
-  Definition loc_350 : location_info := LocationInfo file_0 121 2 123 3.
-  Definition loc_351 : location_info := LocationInfo file_0 121 31 123 3.
-  Definition loc_352 : location_info := LocationInfo file_0 122 4 122 26.
-  Definition loc_353 : location_info := LocationInfo file_0 121 2 123 3.
-  Definition loc_354 : location_info := LocationInfo file_0 121 2 123 3.
-  Definition loc_355 : location_info := LocationInfo file_0 122 4 122 7.
-  Definition loc_356 : location_info := LocationInfo file_0 122 10 122 25.
-  Definition loc_357 : location_info := LocationInfo file_0 122 11 122 25.
-  Definition loc_358 : location_info := LocationInfo file_0 122 12 122 18.
-  Definition loc_359 : location_info := LocationInfo file_0 122 12 122 18.
-  Definition loc_360 : location_info := LocationInfo file_0 122 14 122 17.
-  Definition loc_361 : location_info := LocationInfo file_0 122 14 122 17.
-  Definition loc_362 : location_info := LocationInfo file_0 121 8 121 30.
-  Definition loc_363 : location_info := LocationInfo file_0 121 8 121 12.
-  Definition loc_364 : location_info := LocationInfo file_0 121 8 121 12.
-  Definition loc_365 : location_info := LocationInfo file_0 121 9 121 12.
-  Definition loc_366 : location_info := LocationInfo file_0 121 9 121 12.
-  Definition loc_367 : location_info := LocationInfo file_0 121 16 121 30.
-  Definition loc_368 : location_info := LocationInfo file_0 117 16 117 18.
-  Definition loc_369 : location_info := LocationInfo file_0 117 16 117 18.
-  Definition loc_374 : location_info := LocationInfo file_0 134 4 134 21.
-  Definition loc_375 : location_info := LocationInfo file_0 139 4 148 5.
-  Definition loc_376 : location_info := LocationInfo file_0 149 4 149 13.
-  Definition loc_377 : location_info := LocationInfo file_0 149 11 149 12.
-  Definition loc_378 : location_info := LocationInfo file_0 139 4 148 5.
-  Definition loc_379 : location_info := LocationInfo file_0 139 35 148 5.
-  Definition loc_380 : location_info := LocationInfo file_0 140 8 140 27.
-  Definition loc_381 : location_info := LocationInfo file_0 142 8 142 33.
-  Definition loc_382 : location_info := LocationInfo file_0 143 8 145 9.
-  Definition loc_383 : location_info := LocationInfo file_0 147 8 147 26.
-  Definition loc_384 : location_info := LocationInfo file_0 139 4 148 5.
-  Definition loc_385 : location_info := LocationInfo file_0 139 4 148 5.
-  Definition loc_386 : location_info := LocationInfo file_0 147 8 147 12.
-  Definition loc_387 : location_info := LocationInfo file_0 147 15 147 25.
-  Definition loc_388 : location_info := LocationInfo file_0 147 16 147 25.
-  Definition loc_389 : location_info := LocationInfo file_0 147 16 147 19.
-  Definition loc_390 : location_info := LocationInfo file_0 147 16 147 19.
-  Definition loc_391 : location_info := LocationInfo file_0 143 23 145 9.
-  Definition loc_392 : location_info := LocationInfo file_0 144 12 144 21.
-  Definition loc_393 : location_info := LocationInfo file_0 144 19 144 20.
-  Definition loc_395 : location_info := LocationInfo file_0 143 11 143 21.
-  Definition loc_396 : location_info := LocationInfo file_0 143 11 143 16.
-  Definition loc_397 : location_info := LocationInfo file_0 143 11 143 16.
-  Definition loc_398 : location_info := LocationInfo file_0 143 12 143 16.
-  Definition loc_399 : location_info := LocationInfo file_0 143 12 143 16.
-  Definition loc_400 : location_info := LocationInfo file_0 143 20 143 21.
-  Definition loc_401 : location_info := LocationInfo file_0 143 20 143 21.
-  Definition loc_402 : location_info := LocationInfo file_0 142 23 142 32.
-  Definition loc_403 : location_info := LocationInfo file_0 142 23 142 32.
-  Definition loc_404 : location_info := LocationInfo file_0 142 23 142 26.
-  Definition loc_405 : location_info := LocationInfo file_0 142 23 142 26.
-  Definition loc_408 : location_info := LocationInfo file_0 140 21 140 26.
-  Definition loc_409 : location_info := LocationInfo file_0 140 21 140 26.
-  Definition loc_410 : location_info := LocationInfo file_0 140 22 140 26.
-  Definition loc_411 : location_info := LocationInfo file_0 140 22 140 26.
-  Definition loc_414 : location_info := LocationInfo file_0 139 10 139 33.
-  Definition loc_415 : location_info := LocationInfo file_0 139 10 139 15.
-  Definition loc_416 : location_info := LocationInfo file_0 139 10 139 15.
-  Definition loc_417 : location_info := LocationInfo file_0 139 11 139 15.
-  Definition loc_418 : location_info := LocationInfo file_0 139 11 139 15.
-  Definition loc_419 : location_info := LocationInfo file_0 139 19 139 33.
-  Definition loc_420 : location_info := LocationInfo file_0 134 19 134 20.
-  Definition loc_421 : location_info := LocationInfo file_0 134 19 134 20.
-  Definition loc_426 : location_info := LocationInfo file_0 194 2 194 18.
-  Definition loc_427 : location_info := LocationInfo file_0 204 2 209 3.
-  Definition loc_428 : location_info := LocationInfo file_0 204 2 209 3.
-  Definition loc_429 : location_info := LocationInfo file_0 204 31 209 3.
-  Definition loc_430 : location_info := LocationInfo file_0 205 4 205 25.
-  Definition loc_431 : location_info := LocationInfo file_0 206 4 206 20.
-  Definition loc_432 : location_info := LocationInfo file_0 207 4 207 14.
-  Definition loc_433 : location_info := LocationInfo file_0 208 4 208 19.
-  Definition loc_434 : location_info := LocationInfo file_0 204 2 209 3.
-  Definition loc_435 : location_info := LocationInfo file_0 204 2 209 3.
-  Definition loc_436 : location_info := LocationInfo file_0 208 4 208 7.
-  Definition loc_437 : location_info := LocationInfo file_0 208 10 208 18.
-  Definition loc_438 : location_info := LocationInfo file_0 208 10 208 18.
-  Definition loc_439 : location_info := LocationInfo file_0 207 4 207 7.
-  Definition loc_440 : location_info := LocationInfo file_0 207 5 207 7.
-  Definition loc_441 : location_info := LocationInfo file_0 207 5 207 7.
-  Definition loc_442 : location_info := LocationInfo file_0 207 10 207 13.
-  Definition loc_443 : location_info := LocationInfo file_0 207 10 207 13.
-  Definition loc_444 : location_info := LocationInfo file_0 206 4 206 13.
-  Definition loc_445 : location_info := LocationInfo file_0 206 4 206 7.
-  Definition loc_446 : location_info := LocationInfo file_0 206 4 206 7.
-  Definition loc_447 : location_info := LocationInfo file_0 206 16 206 19.
-  Definition loc_448 : location_info := LocationInfo file_0 206 16 206 19.
-  Definition loc_449 : location_info := LocationInfo file_0 206 17 206 19.
-  Definition loc_450 : location_info := LocationInfo file_0 206 17 206 19.
-  Definition loc_451 : location_info := LocationInfo file_0 205 4 205 12.
-  Definition loc_452 : location_info := LocationInfo file_0 205 15 205 24.
-  Definition loc_453 : location_info := LocationInfo file_0 205 15 205 24.
-  Definition loc_454 : location_info := LocationInfo file_0 205 15 205 18.
-  Definition loc_455 : location_info := LocationInfo file_0 205 15 205 18.
-  Definition loc_456 : location_info := LocationInfo file_0 204 8 204 29.
-  Definition loc_457 : location_info := LocationInfo file_0 204 8 204 11.
-  Definition loc_458 : location_info := LocationInfo file_0 204 8 204 11.
-  Definition loc_459 : location_info := LocationInfo file_0 204 15 204 29.
-  Definition loc_460 : location_info := LocationInfo file_0 194 15 194 17.
-  Definition loc_461 : location_info := LocationInfo file_0 194 15 194 17.
+  Definition loc_342 : location_info := LocationInfo file_0 120 2 120 17.
+  Definition loc_343 : location_info := LocationInfo file_0 125 2 128 3.
+  Definition loc_344 : location_info := LocationInfo file_0 129 2 129 13.
+  Definition loc_345 : location_info := LocationInfo file_0 129 9 129 12.
+  Definition loc_346 : location_info := LocationInfo file_0 129 9 129 12.
+  Definition loc_347 : location_info := LocationInfo file_0 125 2 128 3.
+  Definition loc_348 : location_info := LocationInfo file_0 125 30 128 3.
+  Definition loc_349 : location_info := LocationInfo file_0 126 4 126 16.
+  Definition loc_350 : location_info := LocationInfo file_0 127 4 127 13.
+  Definition loc_351 : location_info := LocationInfo file_0 125 2 128 3.
+  Definition loc_352 : location_info := LocationInfo file_0 125 2 128 3.
+  Definition loc_353 : location_info := LocationInfo file_0 127 4 127 7.
+  Definition loc_354 : location_info := LocationInfo file_0 127 4 127 12.
+  Definition loc_355 : location_info := LocationInfo file_0 127 4 127 7.
+  Definition loc_356 : location_info := LocationInfo file_0 127 4 127 7.
+  Definition loc_357 : location_info := LocationInfo file_0 127 11 127 12.
+  Definition loc_358 : location_info := LocationInfo file_0 126 4 126 5.
+  Definition loc_359 : location_info := LocationInfo file_0 126 8 126 15.
+  Definition loc_360 : location_info := LocationInfo file_0 126 8 126 15.
+  Definition loc_361 : location_info := LocationInfo file_0 126 8 126 9.
+  Definition loc_362 : location_info := LocationInfo file_0 126 8 126 9.
+  Definition loc_363 : location_info := LocationInfo file_0 125 9 125 28.
+  Definition loc_364 : location_info := LocationInfo file_0 125 9 125 10.
+  Definition loc_365 : location_info := LocationInfo file_0 125 9 125 10.
+  Definition loc_366 : location_info := LocationInfo file_0 125 14 125 28.
+  Definition loc_367 : location_info := LocationInfo file_0 120 15 120 16.
+  Definition loc_372 : location_info := LocationInfo file_0 136 2 136 19.
+  Definition loc_373 : location_info := LocationInfo file_0 140 2 142 3.
+  Definition loc_374 : location_info := LocationInfo file_0 143 2 143 12.
+  Definition loc_375 : location_info := LocationInfo file_0 143 2 143 6.
+  Definition loc_376 : location_info := LocationInfo file_0 143 3 143 6.
+  Definition loc_377 : location_info := LocationInfo file_0 143 3 143 6.
+  Definition loc_378 : location_info := LocationInfo file_0 143 9 143 11.
+  Definition loc_379 : location_info := LocationInfo file_0 143 9 143 11.
+  Definition loc_380 : location_info := LocationInfo file_0 140 2 142 3.
+  Definition loc_381 : location_info := LocationInfo file_0 140 31 142 3.
+  Definition loc_382 : location_info := LocationInfo file_0 141 4 141 26.
+  Definition loc_383 : location_info := LocationInfo file_0 140 2 142 3.
+  Definition loc_384 : location_info := LocationInfo file_0 140 2 142 3.
+  Definition loc_385 : location_info := LocationInfo file_0 141 4 141 7.
+  Definition loc_386 : location_info := LocationInfo file_0 141 10 141 25.
+  Definition loc_387 : location_info := LocationInfo file_0 141 11 141 25.
+  Definition loc_388 : location_info := LocationInfo file_0 141 12 141 18.
+  Definition loc_389 : location_info := LocationInfo file_0 141 12 141 18.
+  Definition loc_390 : location_info := LocationInfo file_0 141 14 141 17.
+  Definition loc_391 : location_info := LocationInfo file_0 141 14 141 17.
+  Definition loc_392 : location_info := LocationInfo file_0 140 8 140 30.
+  Definition loc_393 : location_info := LocationInfo file_0 140 8 140 12.
+  Definition loc_394 : location_info := LocationInfo file_0 140 8 140 12.
+  Definition loc_395 : location_info := LocationInfo file_0 140 9 140 12.
+  Definition loc_396 : location_info := LocationInfo file_0 140 9 140 12.
+  Definition loc_397 : location_info := LocationInfo file_0 140 16 140 30.
+  Definition loc_398 : location_info := LocationInfo file_0 136 16 136 18.
+  Definition loc_399 : location_info := LocationInfo file_0 136 16 136 18.
+  Definition loc_404 : location_info := LocationInfo file_0 153 4 153 21.
+  Definition loc_405 : location_info := LocationInfo file_0 158 4 167 5.
+  Definition loc_406 : location_info := LocationInfo file_0 168 4 168 13.
+  Definition loc_407 : location_info := LocationInfo file_0 168 11 168 12.
+  Definition loc_408 : location_info := LocationInfo file_0 158 4 167 5.
+  Definition loc_409 : location_info := LocationInfo file_0 158 35 167 5.
+  Definition loc_410 : location_info := LocationInfo file_0 159 8 159 27.
+  Definition loc_411 : location_info := LocationInfo file_0 161 8 161 33.
+  Definition loc_412 : location_info := LocationInfo file_0 162 8 164 9.
+  Definition loc_413 : location_info := LocationInfo file_0 166 8 166 26.
+  Definition loc_414 : location_info := LocationInfo file_0 158 4 167 5.
+  Definition loc_415 : location_info := LocationInfo file_0 158 4 167 5.
+  Definition loc_416 : location_info := LocationInfo file_0 166 8 166 12.
+  Definition loc_417 : location_info := LocationInfo file_0 166 15 166 25.
+  Definition loc_418 : location_info := LocationInfo file_0 166 16 166 25.
+  Definition loc_419 : location_info := LocationInfo file_0 166 16 166 19.
+  Definition loc_420 : location_info := LocationInfo file_0 166 16 166 19.
+  Definition loc_421 : location_info := LocationInfo file_0 162 23 164 9.
+  Definition loc_422 : location_info := LocationInfo file_0 163 12 163 21.
+  Definition loc_423 : location_info := LocationInfo file_0 163 19 163 20.
+  Definition loc_425 : location_info := LocationInfo file_0 162 11 162 21.
+  Definition loc_426 : location_info := LocationInfo file_0 162 11 162 16.
+  Definition loc_427 : location_info := LocationInfo file_0 162 11 162 16.
+  Definition loc_428 : location_info := LocationInfo file_0 162 12 162 16.
+  Definition loc_429 : location_info := LocationInfo file_0 162 12 162 16.
+  Definition loc_430 : location_info := LocationInfo file_0 162 20 162 21.
+  Definition loc_431 : location_info := LocationInfo file_0 162 20 162 21.
+  Definition loc_432 : location_info := LocationInfo file_0 161 23 161 32.
+  Definition loc_433 : location_info := LocationInfo file_0 161 23 161 32.
+  Definition loc_434 : location_info := LocationInfo file_0 161 23 161 26.
+  Definition loc_435 : location_info := LocationInfo file_0 161 23 161 26.
+  Definition loc_438 : location_info := LocationInfo file_0 159 21 159 26.
+  Definition loc_439 : location_info := LocationInfo file_0 159 21 159 26.
+  Definition loc_440 : location_info := LocationInfo file_0 159 22 159 26.
+  Definition loc_441 : location_info := LocationInfo file_0 159 22 159 26.
+  Definition loc_444 : location_info := LocationInfo file_0 158 10 158 33.
+  Definition loc_445 : location_info := LocationInfo file_0 158 10 158 15.
+  Definition loc_446 : location_info := LocationInfo file_0 158 10 158 15.
+  Definition loc_447 : location_info := LocationInfo file_0 158 11 158 15.
+  Definition loc_448 : location_info := LocationInfo file_0 158 11 158 15.
+  Definition loc_449 : location_info := LocationInfo file_0 158 19 158 33.
+  Definition loc_450 : location_info := LocationInfo file_0 153 19 153 20.
+  Definition loc_451 : location_info := LocationInfo file_0 153 19 153 20.
+  Definition loc_456 : location_info := LocationInfo file_0 213 2 213 18.
+  Definition loc_457 : location_info := LocationInfo file_0 223 2 228 3.
+  Definition loc_458 : location_info := LocationInfo file_0 223 2 228 3.
+  Definition loc_459 : location_info := LocationInfo file_0 223 31 228 3.
+  Definition loc_460 : location_info := LocationInfo file_0 224 4 224 25.
+  Definition loc_461 : location_info := LocationInfo file_0 225 4 225 20.
+  Definition loc_462 : location_info := LocationInfo file_0 226 4 226 14.
+  Definition loc_463 : location_info := LocationInfo file_0 227 4 227 19.
+  Definition loc_464 : location_info := LocationInfo file_0 223 2 228 3.
+  Definition loc_465 : location_info := LocationInfo file_0 223 2 228 3.
+  Definition loc_466 : location_info := LocationInfo file_0 227 4 227 7.
+  Definition loc_467 : location_info := LocationInfo file_0 227 10 227 18.
+  Definition loc_468 : location_info := LocationInfo file_0 227 10 227 18.
+  Definition loc_469 : location_info := LocationInfo file_0 226 4 226 7.
+  Definition loc_470 : location_info := LocationInfo file_0 226 5 226 7.
+  Definition loc_471 : location_info := LocationInfo file_0 226 5 226 7.
+  Definition loc_472 : location_info := LocationInfo file_0 226 10 226 13.
+  Definition loc_473 : location_info := LocationInfo file_0 226 10 226 13.
+  Definition loc_474 : location_info := LocationInfo file_0 225 4 225 13.
+  Definition loc_475 : location_info := LocationInfo file_0 225 4 225 7.
+  Definition loc_476 : location_info := LocationInfo file_0 225 4 225 7.
+  Definition loc_477 : location_info := LocationInfo file_0 225 16 225 19.
+  Definition loc_478 : location_info := LocationInfo file_0 225 16 225 19.
+  Definition loc_479 : location_info := LocationInfo file_0 225 17 225 19.
+  Definition loc_480 : location_info := LocationInfo file_0 225 17 225 19.
+  Definition loc_481 : location_info := LocationInfo file_0 224 4 224 12.
+  Definition loc_482 : location_info := LocationInfo file_0 224 15 224 24.
+  Definition loc_483 : location_info := LocationInfo file_0 224 15 224 24.
+  Definition loc_484 : location_info := LocationInfo file_0 224 15 224 18.
+  Definition loc_485 : location_info := LocationInfo file_0 224 15 224 18.
+  Definition loc_486 : location_info := LocationInfo file_0 223 8 223 29.
+  Definition loc_487 : location_info := LocationInfo file_0 223 8 223 11.
+  Definition loc_488 : location_info := LocationInfo file_0 223 8 223 11.
+  Definition loc_489 : location_info := LocationInfo file_0 223 15 223 29.
+  Definition loc_490 : location_info := LocationInfo file_0 213 15 213 17.
+  Definition loc_491 : location_info := LocationInfo file_0 213 15 213 17.
 
   (* Definition of struct [list]. *)
   Program Definition struct_list := {|
@@ -795,6 +821,53 @@ Section code.
     )%E
   |}.
 
+  (* Definition of function [length_val]. *)
+  Definition impl_length_val : function := {|
+    f_args := [
+      ("p", LPtr)
+    ];
+    f_local_vars := [
+      ("len", it_layout size_t)
+    ];
+    f_init := "#0";
+    f_code := (
+      <[ "#0" :=
+        "len" <-{ it_layout size_t }
+          LocInfoE loc_367 (UnOp (CastOp $ IntOp size_t) (IntOp i32) (LocInfoE loc_367 (i2v 0 i32))) ;
+        locinfo: loc_343 ;
+        Goto "#1"
+      ]> $
+      <[ "#1" :=
+        locinfo: loc_363 ;
+        if: LocInfoE loc_363 (UnOp (CastOp $ IntOp bool_it) (IntOp i32) (LocInfoE loc_363 ((LocInfoE loc_364 (use{LPtr} (LocInfoE loc_365 ("p")))) !={PtrOp, PtrOp} (LocInfoE loc_366 (NULL)))))
+        then
+        locinfo: loc_349 ;
+          Goto "#2"
+        else
+        locinfo: loc_344 ;
+          Goto "#3"
+      ]> $
+      <[ "#2" :=
+        locinfo: loc_349 ;
+        LocInfoE loc_358 ("p") <-{ LPtr }
+          LocInfoE loc_359 (use{LPtr} (LocInfoE loc_360 ((LocInfoE loc_361 (!{LPtr} (LocInfoE loc_362 ("p")))) at{struct_list} "tail"))) ;
+        locinfo: loc_350 ;
+        LocInfoE loc_353 ("len") <-{ it_layout size_t }
+          LocInfoE loc_354 ((LocInfoE loc_355 (use{it_layout size_t} (LocInfoE loc_356 ("len")))) +{IntOp size_t, IntOp size_t} (LocInfoE loc_357 (UnOp (CastOp $ IntOp size_t) (IntOp i32) (LocInfoE loc_357 (i2v 1 i32))))) ;
+        locinfo: loc_351 ;
+        Goto "continue22"
+      ]> $
+      <[ "#3" :=
+        locinfo: loc_344 ;
+        Return (LocInfoE loc_345 (use{it_layout size_t} (LocInfoE loc_346 ("len"))))
+      ]> $
+      <[ "continue22" :=
+        locinfo: loc_343 ;
+        Goto "#1"
+      ]> $∅
+    )%E
+  |}.
+
   (* Definition of function [append]. *)
   Definition impl_append : function := {|
     f_args := [
@@ -808,35 +881,35 @@ Section code.
     f_code := (
       <[ "#0" :=
         "end" <-{ LPtr }
-          LocInfoE loc_368 (use{LPtr} (LocInfoE loc_369 ("l1"))) ;
-        locinfo: loc_343 ;
+          LocInfoE loc_398 (use{LPtr} (LocInfoE loc_399 ("l1"))) ;
+        locinfo: loc_373 ;
         Goto "#1"
       ]> $
       <[ "#1" :=
-        locinfo: loc_362 ;
-        if: LocInfoE loc_362 (UnOp (CastOp $ IntOp bool_it) (IntOp i32) (LocInfoE loc_362 ((LocInfoE loc_363 (use{LPtr} (LocInfoE loc_365 (!{LPtr} (LocInfoE loc_366 ("end")))))) !={PtrOp, PtrOp} (LocInfoE loc_367 (NULL)))))
+        locinfo: loc_392 ;
+        if: LocInfoE loc_392 (UnOp (CastOp $ IntOp bool_it) (IntOp i32) (LocInfoE loc_392 ((LocInfoE loc_393 (use{LPtr} (LocInfoE loc_395 (!{LPtr} (LocInfoE loc_396 ("end")))))) !={PtrOp, PtrOp} (LocInfoE loc_397 (NULL)))))
         then
-        locinfo: loc_352 ;
+        locinfo: loc_382 ;
           Goto "#2"
         else
-        locinfo: loc_344 ;
+        locinfo: loc_374 ;
           Goto "#3"
       ]> $
       <[ "#2" :=
-        locinfo: loc_352 ;
-        LocInfoE loc_355 ("end") <-{ LPtr }
-          LocInfoE loc_356 (&(LocInfoE loc_357 ((LocInfoE loc_358 (!{LPtr} (LocInfoE loc_360 (!{LPtr} (LocInfoE loc_361 ("end")))))) at{struct_list} "tail"))) ;
-        locinfo: loc_353 ;
-        Goto "continue22"
+        locinfo: loc_382 ;
+        LocInfoE loc_385 ("end") <-{ LPtr }
+          LocInfoE loc_386 (&(LocInfoE loc_387 ((LocInfoE loc_388 (!{LPtr} (LocInfoE loc_390 (!{LPtr} (LocInfoE loc_391 ("end")))))) at{struct_list} "tail"))) ;
+        locinfo: loc_383 ;
+        Goto "continue26"
       ]> $
       <[ "#3" :=
-        locinfo: loc_344 ;
-        LocInfoE loc_346 (!{LPtr} (LocInfoE loc_347 ("end"))) <-{ LPtr }
-          LocInfoE loc_348 (use{LPtr} (LocInfoE loc_349 ("l2"))) ;
+        locinfo: loc_374 ;
+        LocInfoE loc_376 (!{LPtr} (LocInfoE loc_377 ("end"))) <-{ LPtr }
+          LocInfoE loc_378 (use{LPtr} (LocInfoE loc_379 ("l2"))) ;
         Return (VOID)
       ]> $
-      <[ "continue22" :=
-        locinfo: loc_343 ;
+      <[ "continue26" :=
+        locinfo: loc_373 ;
         Goto "#1"
       ]> $∅
     )%E
@@ -857,54 +930,54 @@ Section code.
     f_code := (
       <[ "#0" :=
         "prev" <-{ LPtr }
-          LocInfoE loc_420 (use{LPtr} (LocInfoE loc_421 ("p"))) ;
-        locinfo: loc_375 ;
+          LocInfoE loc_450 (use{LPtr} (LocInfoE loc_451 ("p"))) ;
+        locinfo: loc_405 ;
         Goto "#1"
       ]> $
       <[ "#1" :=
-        locinfo: loc_414 ;
-        if: LocInfoE loc_414 (UnOp (CastOp $ IntOp bool_it) (IntOp i32) (LocInfoE loc_414 ((LocInfoE loc_415 (use{LPtr} (LocInfoE loc_417 (!{LPtr} (LocInfoE loc_418 ("prev")))))) !={PtrOp, PtrOp} (LocInfoE loc_419 (NULL)))))
+        locinfo: loc_444 ;
+        if: LocInfoE loc_444 (UnOp (CastOp $ IntOp bool_it) (IntOp i32) (LocInfoE loc_444 ((LocInfoE loc_445 (use{LPtr} (LocInfoE loc_447 (!{LPtr} (LocInfoE loc_448 ("prev")))))) !={PtrOp, PtrOp} (LocInfoE loc_449 (NULL)))))
         then
         Goto "#2"
         else
-        locinfo: loc_376 ;
+        locinfo: loc_406 ;
           Goto "#3"
       ]> $
       <[ "#2" :=
         "cur" <-{ LPtr }
-          LocInfoE loc_408 (use{LPtr} (LocInfoE loc_410 (!{LPtr} (LocInfoE loc_411 ("prev"))))) ;
+          LocInfoE loc_438 (use{LPtr} (LocInfoE loc_440 (!{LPtr} (LocInfoE loc_441 ("prev"))))) ;
         "head" <-{ LPtr }
-          LocInfoE loc_402 (UnOp (CastOp $ PtrOp) (PtrOp) (LocInfoE loc_402 (use{LPtr} (LocInfoE loc_403 ((LocInfoE loc_404 (!{LPtr} (LocInfoE loc_405 ("cur")))) at{struct_list} "head"))))) ;
-        locinfo: loc_395 ;
-        if: LocInfoE loc_395 (UnOp (CastOp $ IntOp bool_it) (IntOp i32) (LocInfoE loc_395 ((LocInfoE loc_396 (use{it_layout size_t} (LocInfoE loc_398 (!{LPtr} (LocInfoE loc_399 ("head")))))) ={IntOp size_t, IntOp size_t} (LocInfoE loc_400 (use{it_layout size_t} (LocInfoE loc_401 ("k")))))))
+          LocInfoE loc_432 (UnOp (CastOp $ PtrOp) (PtrOp) (LocInfoE loc_432 (use{LPtr} (LocInfoE loc_433 ((LocInfoE loc_434 (!{LPtr} (LocInfoE loc_435 ("cur")))) at{struct_list} "head"))))) ;
+        locinfo: loc_425 ;
+        if: LocInfoE loc_425 (UnOp (CastOp $ IntOp bool_it) (IntOp i32) (LocInfoE loc_425 ((LocInfoE loc_426 (use{it_layout size_t} (LocInfoE loc_428 (!{LPtr} (LocInfoE loc_429 ("head")))))) ={IntOp size_t, IntOp size_t} (LocInfoE loc_430 (use{it_layout size_t} (LocInfoE loc_431 ("k")))))))
         then
-        locinfo: loc_392 ;
+        locinfo: loc_422 ;
           Goto "#5"
         else
-        locinfo: loc_383 ;
+        locinfo: loc_413 ;
           Goto "#6"
       ]> $
       <[ "#3" :=
-        locinfo: loc_376 ;
-        Return (LocInfoE loc_377 (UnOp (CastOp $ IntOp bool_it) (IntOp i32) (LocInfoE loc_377 (i2v 0 i32))))
+        locinfo: loc_406 ;
+        Return (LocInfoE loc_407 (UnOp (CastOp $ IntOp bool_it) (IntOp i32) (LocInfoE loc_407 (i2v 0 i32))))
       ]> $
       <[ "#4" :=
-        locinfo: loc_383 ;
-        LocInfoE loc_386 ("prev") <-{ LPtr }
-          LocInfoE loc_387 (&(LocInfoE loc_388 ((LocInfoE loc_389 (!{LPtr} (LocInfoE loc_390 ("cur")))) at{struct_list} "tail"))) ;
-        locinfo: loc_384 ;
-        Goto "continue26"
+        locinfo: loc_413 ;
+        LocInfoE loc_416 ("prev") <-{ LPtr }
+          LocInfoE loc_417 (&(LocInfoE loc_418 ((LocInfoE loc_419 (!{LPtr} (LocInfoE loc_420 ("cur")))) at{struct_list} "tail"))) ;
+        locinfo: loc_414 ;
+        Goto "continue30"
       ]> $
       <[ "#5" :=
-        locinfo: loc_392 ;
-        Return (LocInfoE loc_393 (UnOp (CastOp $ IntOp bool_it) (IntOp i32) (LocInfoE loc_393 (i2v 1 i32))))
+        locinfo: loc_422 ;
+        Return (LocInfoE loc_423 (UnOp (CastOp $ IntOp bool_it) (IntOp i32) (LocInfoE loc_423 (i2v 1 i32))))
       ]> $
       <[ "#6" :=
-        locinfo: loc_383 ;
+        locinfo: loc_413 ;
         Goto "#4"
       ]> $
-      <[ "continue26" :=
-        locinfo: loc_375 ;
+      <[ "continue30" :=
+        locinfo: loc_405 ;
         Goto "#1"
       ]> $∅
     )%E
@@ -924,40 +997,40 @@ Section code.
     f_code := (
       <[ "#0" :=
         "cur" <-{ LPtr }
-          LocInfoE loc_460 (use{LPtr} (LocInfoE loc_461 ("l1"))) ;
-        locinfo: loc_427 ;
+          LocInfoE loc_490 (use{LPtr} (LocInfoE loc_491 ("l1"))) ;
+        locinfo: loc_457 ;
         Goto "#1"
       ]> $
       <[ "#1" :=
-        locinfo: loc_456 ;
-        if: LocInfoE loc_456 (UnOp (CastOp $ IntOp bool_it) (IntOp i32) (LocInfoE loc_456 ((LocInfoE loc_457 (use{LPtr} (LocInfoE loc_458 ("cur")))) !={PtrOp, PtrOp} (LocInfoE loc_459 (NULL)))))
+        locinfo: loc_486 ;
+        if: LocInfoE loc_486 (UnOp (CastOp $ IntOp bool_it) (IntOp i32) (LocInfoE loc_486 ((LocInfoE loc_487 (use{LPtr} (LocInfoE loc_488 ("cur")))) !={PtrOp, PtrOp} (LocInfoE loc_489 (NULL)))))
         then
-        locinfo: loc_430 ;
+        locinfo: loc_460 ;
           Goto "#2"
         else
         Goto "#3"
       ]> $
       <[ "#2" :=
-        locinfo: loc_430 ;
-        LocInfoE loc_451 ("cur_tail") <-{ LPtr }
-          LocInfoE loc_452 (use{LPtr} (LocInfoE loc_453 ((LocInfoE loc_454 (!{LPtr} (LocInfoE loc_455 ("cur")))) at{struct_list} "tail"))) ;
-        locinfo: loc_431 ;
-        LocInfoE loc_444 ((LocInfoE loc_445 (!{LPtr} (LocInfoE loc_446 ("cur")))) at{struct_list} "tail") <-{ LPtr }
-          LocInfoE loc_447 (use{LPtr} (LocInfoE loc_449 (!{LPtr} (LocInfoE loc_450 ("l2"))))) ;
-        locinfo: loc_432 ;
-        LocInfoE loc_440 (!{LPtr} (LocInfoE loc_441 ("l2"))) <-{ LPtr }
-          LocInfoE loc_442 (use{LPtr} (LocInfoE loc_443 ("cur"))) ;
-        locinfo: loc_433 ;
-        LocInfoE loc_436 ("cur") <-{ LPtr }
-          LocInfoE loc_437 (use{LPtr} (LocInfoE loc_438 ("cur_tail"))) ;
-        locinfo: loc_434 ;
-        Goto "continue33"
+        locinfo: loc_460 ;
+        LocInfoE loc_481 ("cur_tail") <-{ LPtr }
+          LocInfoE loc_482 (use{LPtr} (LocInfoE loc_483 ((LocInfoE loc_484 (!{LPtr} (LocInfoE loc_485 ("cur")))) at{struct_list} "tail"))) ;
+        locinfo: loc_461 ;
+        LocInfoE loc_474 ((LocInfoE loc_475 (!{LPtr} (LocInfoE loc_476 ("cur")))) at{struct_list} "tail") <-{ LPtr }
+          LocInfoE loc_477 (use{LPtr} (LocInfoE loc_479 (!{LPtr} (LocInfoE loc_480 ("l2"))))) ;
+        locinfo: loc_462 ;
+        LocInfoE loc_470 (!{LPtr} (LocInfoE loc_471 ("l2"))) <-{ LPtr }
+          LocInfoE loc_472 (use{LPtr} (LocInfoE loc_473 ("cur"))) ;
+        locinfo: loc_463 ;
+        LocInfoE loc_466 ("cur") <-{ LPtr }
+          LocInfoE loc_467 (use{LPtr} (LocInfoE loc_468 ("cur_tail"))) ;
+        locinfo: loc_464 ;
+        Goto "continue37"
       ]> $
       <[ "#3" :=
         Return (VOID)
       ]> $
-      <[ "continue33" :=
-        locinfo: loc_427 ;
+      <[ "continue37" :=
+        locinfo: loc_457 ;
         Goto "#1"
       ]> $∅
     )%E
