tutorial/proofs/t03_list/generated_proof_length_val.v
@@ -1,0 +1,34 @@
+From refinedc.typing Require Import typing.
+From refinedc.tutorial.t03_list Require Import generated_code.
+From refinedc.tutorial.t03_list Require Import generated_spec.
+Set Default Proof Using "Type".
+
+(* Generated from [tutorial/t03_list.c]. *)
+Section proof_length_val.
+  Context `{!typeG Σ} `{!globalG Σ}.
+
+  (* Typing proof for [length_val]. *)
+  Lemma type_length_val :
+    ⊢ typed_function impl_length_val type_of_length_val.
+  Proof.
+    start_function "length_val" ([v l]) => arg_p local_len.
+    split_blocks ((
+      <[ "#1" :=
+        ∃ v2 : val,
+        ∃ l1 : list type,
+        arg_p ◁ₗ (own_constrained (nonshr_constraint (v2 ◁ᵥ l1 @ list_t)) (singleton_val (LPtr) (v2))) ∗
+        local_len ◁ₗ ((length l - length l1) @ (int (size_t))) ∗
+        (v ◁ᵥ wand_val LPtr (v2 ◁ᵥ l1 @ list_t) (l @ list_t))
+    ]> $
+      ∅
+    )%I : gmap label (iProp Σ)) ((
+      ∅
+    )%I : gmap label (iProp Σ)).
+    - repeat liRStep; liShow.
+      all: print_typesystem_goal "length_val" "#0".
+    - repeat liRStep; liShow.
+      all: print_typesystem_goal "length_val" "#1".
+    Unshelve. all: sidecond_hook; prepare_sideconditions; normalize_and_simpl_goal; try solve_goal; unsolved_sidecond_hook.
+    all: print_sidecondition_goal "length_val".
+  Qed.
+End proof_length_val.
